\begin{center}
	\LARGE{\textbf{Ã˜ving 3}}
\end{center}


\section*{11.1}


\subsection*{15}


\begin{gather*}
	f(x) = x^2 \quad
	(0 < x < 2 \pi)
	\\ \\
	a_0 = \frac{1}{2 \pi} \int_0^{2 \pi}{x^2 d x} =
	\frac{1}{2 \pi} \left[\frac{1}{3} x^3\right]_0^{2\pi} =
	\frac{8 \pi^3}{6 \pi} =
	\frac{4}{3} \pi^2
	\\ \\
	a_n = \frac{1}{\pi} \int_0^{2 \pi}{x^2 \cos{n x}\ dx} =
	\frac{1}{\pi} \left[
		\frac{1}{n} x^2 \sin{n x} +
		\frac{2}{n^2} x \cos{n x} -
		\frac{2}{n^3} \sin{n x}
	\right]_0^{2 \pi} =
	\\
	\frac{1}{\pi} \left(
		\frac{4 \pi^2}{n} \cancel{\sin{2 \pi n}} +
		\frac{4 \pi}{n^2} \cos{2 \pi n} -
		\frac{2}{n^3} \cancel{\sin{2 \pi n}}
	\right) -
	\frac{1}{\pi} \left(
		\frac{2}{n^3} \cancel{\sin{0}}
	\right) =
	\frac{4}{n^2}
	\\
	\\
	b_n = \frac{1}{\pi} \int_0^{2 \pi}{x^2 \sin{n x}\ d x} =
	\frac{1}{\pi} \left[
		-\frac{1}{n} x^2 \cos{n x} +
		\frac{2}{n^2} x \sin{n x} +
		\frac{2}{n^3} \cos{n x}
	\right]_0^{2 \pi} =
	\\
	\frac{1}{\pi} \left(
		-\frac{4 \pi^2}{n} \cos{2 \pi n} +
		\cancel{
			\frac{2}{n^3} \cos{2 \pi n} -
			\frac{2}{n^3} \cos{0}
		}
	\right) =
	-\frac{4 \pi}{n}
	\\ \\
	f_N(x) = \frac{4}{3} \pi^2 +
	\sum_{n = 1}^N{\left(
		\frac{4}{n^2} \cos{n x} - \frac{4 \pi}{n} \sin{n x}
	\right)}
\end{gather*}

\bigskip

\plot{Figurer/f0.tikz}{5}{4}
\plot{Figurer/f1.tikz}{5}{4}
\plot{Figurer/f2.tikz}{5}{4}
\bigskip
\\
\plot{Figurer/f3.tikz}{5}{4}
\plot{Figurer/f4.tikz}{5}{4}
\plot{Figurer/f5.tikz}{5}{4}


\newpage


\subsection*{18}


\begin{gather*}
	f(x) = \left\{\begin{matrix*}[l]
		0 &	x < 0 \\
		1 & x > 0
	\end{matrix*}\right. \quad
	-\pi < x < \pi
	\\
	\\
	a_0 = \frac{1}{2 \pi} \int_{-\pi}^\pi{f(x) dx} = \frac{1}{2}
	\\
	\\
	a_n = \frac{1}{\pi} \int_{-\pi}^\pi{f(x) \cos{n x}\ d x} = \frac{1}{\pi} \int_0^\pi{\cos{n x}\ d x} = 0
	\\
	\\
	b_n = \frac{1}{\pi} \int_{-\pi}^\pi{f(x) \sin{n x}\ d x} = \frac{1}{\pi} \int_0^\pi{\sin{n x}\ d x} =
	- \frac{1}{\pi n} \left[
		\cos{n x}
	\right]_0^\pi =
	\\
	- \frac{1}{\pi n} \left(
		\cos{n \pi} - \cos{0}
	\right) =
	- \frac{1}{\pi n} \left(
		(-1)^n - 1
	\right) \\
	b_n = \left\{\begin{matrix*}[l]
		\frac{2}{\pi n}	& n\ \text{odd} \\
		0					& n\ \text{even}
	\end{matrix*}\right.
	\\
	\\
	f_N(x) = \frac{1}{2} + \sum_{n = 1}^{\lceil N / 2 \rceil}{\left(
		\frac{2}{\pi (2 n - 1)} \sin{n x}
	\right)}
\end{gather*}

\bigskip

\plot{Figurer/g0.tikz}{5}{4}
\plot{Figurer/g1.tikz}{5}{4}
\plot{Figurer/g3.tikz}{5}{4}
\bigskip
\\
\plot{Figurer/g5.tikz}{5}{4}
\plot{Figurer/g7.tikz}{5}{4}
\plot{Figurer/g9.tikz}{5}{4}


\newpage

\subsection*{20}


\begin{gather*}
	f(x) = \left\{\begin{matrix*}[l]
		-\frac{\pi}{2}	& x < -\frac{\pi}{2} \\
		x				& -\frac{\pi}{2} \leq x \leq \frac{\pi}{2} \\
		\frac{\pi}{2}	& \frac{\pi}{2} < x
	\end{matrix*}\right.
	\\
	\\
	f(x)\ \text{odd} \Rightarrow a_n = 0 \quad \forall \quad n \in \mathbb{N}
	\\
	b_n = \frac{1}{\pi} \int_{-\pi}^\pi{f(x) \sin{n x}\ d x} =
	\frac{2}{\pi} \int_0^\pi{f(x) \sin{n x}\ d x} =
	\\
	\frac{2}{\pi} \int_0^{\frac{\pi}{2}}{x \sin{n x}\ d x} +
	\frac{2}{\pi} \int_{\frac{\pi}{2}}^\pi{\frac{\pi}{2} \sin{n x}\ d x} =
	\\
	\frac{2}{\pi} \left[
		-\frac{1}{n} x \cos{n x} +
		\frac{1}{n^2} \sin{n x}
	\right]_0^{\frac{\pi}{2}} +
	\left[
		-\frac{1}{n}\cos{n x}
	\right]_\frac{\pi}{2}^\pi =
	\\
	\frac{2}{\pi} \left(
		- \cancel{\frac{\pi}{2 n} \cos{\frac{n \pi}{2}}} +
		\frac{1}{n^2} \sin{\frac{n \pi}{2}}
	\right) +
	\cancel{\frac{1}{n} \cos{\frac{n \pi}{2}}} -
	\frac{1}{n} \cos{n \pi}
	\\
	\\
	b_n = \left\{\begin{matrix*}[l]
		-\frac{1}{n}											& n\ \text{even} \\
		\frac{2 (-1)^{\frac{n - 1}{2}}}{\pi n^2} + \frac{1}{n}	& n\ \text{odd}
	\end{matrix*}\right.
	\\
	\\
	f_N(x) = \sum_{n\ \text{odd}}^{N}{\left(
		\frac{2 (-1)^{\frac{n - 1}{2}}}{\pi n^2} + \frac{1}{n}
	\right)
	\sin{n x}} -
	\sum_{n\ \text{even}}^N{\frac{1}{n} \sin{n x}}
\end{gather*}


\plot{Figurer/h0.tikz}{5}{4}
\plot{Figurer/h1.tikz}{5}{4}
\plot{Figurer/h2.tikz}{5}{4}
\bigskip
\\
\plot{Figurer/h3.tikz}{5}{4}
\plot{Figurer/h4.tikz}{5}{4}
\plot{Figurer/h5.tikz}{5}{4}


\newpage

\section*{11.2}


\subsection*{9}


\begin{gather*}
	f(x) = \left\{\begin{matrix*}[l]
		-1	& x < 0 \\
		1	& x > 0
	\end{matrix*}\right.
	\\
	f(-x) = \left\{\begin{matrix*}[l]
		-1	& (-x) < 0 \\
		1	& (-x) > 0
	\end{matrix*}\right. =
	\left\{\begin{matrix*}[l]
		-1	& x > 0 \\
		1	& x < 0
	\end{matrix*}\right. =
	\\
	\left\{\begin{matrix*}[l]
		1	& x < 0 \\
		-1	& x > 0
	\end{matrix*}\right. =
	- \left\{\begin{matrix*}[l]
		-1	& x < 0 \\
		1	& x > 0
	\end{matrix*}\right. =
	-f(x) \Rightarrow \\
	f(x)\ \text{is odd}
	\\
	\\
	a_n = 0, \quad
	b_n = \frac{2}{2} \int_0^2{\sin{\frac{\pi n x}{2}}\ d x} =
	\left[
		-\frac{2}{\pi n} \cos{\frac{\pi n x}{2}}
	\right]_0^2 =
	\frac{2}{\pi} \left(
		-\frac{1}{n} \cos{n \pi} +
		\frac{1}{n}
	\right)
	\\
	\frac{2}{\pi n} \left(
		1 - (-1)^{n + 1}
	\right) =
	\left\{\begin{matrix*}[l]
		\frac{4}{\pi n}	& n\ \text{odd} \\
		0				& n\ \text{even}
	\end{matrix*}
	\right.
	\\
	\\
	f_N(x) = \sum_{n\ \text{odd}}^N{\left(\frac{4}{\pi n} \sin{\frac{\pi n x}{2}}\right)}
\end{gather*}
\bigskip

\plot{Figurer/j0.tikz}{5}{4}
\plot{Figurer/j1.tikz}{5}{4}
\plot{Figurer/j2.tikz}{5}{4}
\bigskip
\\
\plot{Figurer/j3.tikz}{5}{4}
\plot{Figurer/j4.tikz}{5}{4}
\plot{Figurer/j5.tikz}{5}{4}


\newpage


\subsection*{15}


\begin{gather*}
	f(x) =
	\left\{\begin{matrix*}[l]
		-x - \pi	& x < -\frac{\pi}{2} \\
		x			& -\frac{\pi}{2} < x < \frac{\pi}{2} \\
		-x + \pi	& \frac{\pi}{2} < x
	\end{matrix*}\right.
	\\
	f(-x) =
	\left\{\begin{matrix*}[l]
		x - \pi	& -x < -\frac{\pi}{2} \\
		-x			& -\frac{\pi}{2} < -x < \frac{\pi}{2} \\
		x + \pi	& \frac{\pi}{2} < -x
	\end{matrix*}\right. =
	\left\{\begin{matrix*}[l]
		x - \pi	& x > \frac{\pi}{2} \\
		-x			& \frac{\pi}{2} > x > -\frac{\pi}{2} \\
		x + \pi	& -\frac{\pi}{2} > x
	\end{matrix*}\right. =
	\\
	\left\{\begin{matrix*}[l]
		x - \pi	& \frac{\pi}{2} < x \\
		-x			& -\frac{\pi}{2} < x < \frac{\pi}{2} \\
		x + \pi	& x < -\frac{\pi}{2}
	\end{matrix*}\right. =
	\left\{\begin{matrix*}[l]
		x + \pi	& x < -\frac{\pi}{2} \\
		-x			& -\frac{\pi}{2} < x < \frac{\pi}{2} \\
		x - \pi	& \frac{\pi}{2} < x
	\end{matrix*}\right. =
	\\
	-\left\{\begin{matrix*}[l]
		-x - \pi	& x < -\frac{\pi}{2} \\
		x			& -\frac{\pi}{2} < x < \frac{\pi}{2} \\
		-x + \pi	& \frac{\pi}{2} < x
	\end{matrix*}\right. = -f(x) \Rightarrow
	\\
	f(x)\ \text{is odd}
	\\
	\\
	a_n = 0, \quad
	b_n = \frac{2}{\pi} \int_0^\pi{f(x) \sin{n x}\ dx} =
	\\
	\frac{2}{\pi} \int_0^{\frac{\pi}{2}}{x \sin{n x}\ dx} +
	\frac{2}{\pi} \int_{\frac{\pi}{2}}^\pi{\left(
		\pi \sin{n x} -
		x \sin{n x}
	\right) dx} =
	\\
	\frac{2}{\pi}
	\left(
		\left[
			\frac{1}{n^2} \sin{n x} - \frac{x}{n} \cos{n x}
		\right]_0^{\frac{\pi}{2}}
		+
		\left[
			-\frac{\pi}{n} \cos{n x} +
			\frac{x}{n} \cos{n x}
			-
			\frac{1}{n^2} \sin{n x}
		\right]_\frac{\pi}{2}^\pi
	\right) =
	\\
	\frac{2}{\pi n^2}
	\left(
		2 \sin{n \frac{\pi}{2}} -
		\sin{n \pi}
	\right) =
	\left\{
		\begin{matrix*}[l]
			\frac{4}{\pi n^2} (-1)^{\frac{n - 1}{2}}	& n\ \text{odd} \\ \\
			0											& n\ \text{even}
		\end{matrix*}
	\right.
	\\
	f_N(x) = \sum_{n\ \text{odd}}^N{
		\frac{4}{\pi n^2} (-1)^{\frac{n - 1}{2}} \sin{n x}
	}
\end{gather*}


\bigskip

\plot{Figurer/i1.tikz}{5}{4}
\plot{Figurer/i2.tikz}{5}{4}
\plot{Figurer/i3.tikz}{5}{4}


\newpage


\subsection*{29}


\begin{gather*}
	\text{Fourier sine series for } \sin{x} = \sin{x}
	\\
	\\
	a_0 = \frac{1}{\pi} \int_0^\pi{\sin{x}\ dx} =
	\frac{1}{\pi} \left[
		-\cos{x}
	\right]_0^\pi =
	\frac{2}{\pi}
	\\
	\\
	a_n = \frac{2}{\pi} \int_0^\pi{
		\sin{x} \cos{n x}\ dx
	} =
	\frac{2}{\pi \left(n^2 - 1\right)}
	\left[
		\cos{x} \cos{n x} + n \sin{x} \sin{n x}
	\right]_0^\pi =
	\\
	\frac{2}{\pi \left(n^2 - 1\right)}
	\left(
		-\cos{n \pi} - 1
	\right) =
	\left\{
		\begin{matrix*}
			\frac{4}{\pi \left(1 - n^2\right)}	& n\ \text{even} \\ \\
			0									& n\ \text{odd}
		\end{matrix*}
	\right.
	\\
	\\
	f_N(x) = \frac{2}{\pi} + \sum_{n\ \text{even}}^N{\frac{4}{\pi \left(1 - n^2\right)} \cos{n x}}
\end{gather*}

\bigskip

\plot{Figurer/k0.tikz}{5}{4}
\plot{Figurer/k1.tikz}{5}{4}
\plot{Figurer/k2.tikz}{5}{4}
\bigskip
\\
\plot{Figurer/k3.tikz}{5}{4}
\plot{Figurer/k4.tikz}{5}{4}
\plot{Figurer/k5.tikz}{5}{4}

