\begin{center}
	\LARGE{\textbf{Ã˜ving 7}}
\end{center}


% \section{12.1.15}

% \begin{gather*}
	
% \end{gather*}


\section*{12.4}

\subsection*{19}


\begin{gather*}
	u_{tt} = c^2 u_{xx}
	\qquad
	u(0, t) = 0
	\qquad
	u_x(L, t) = 0
	\\
	\\
	u_n(x, t) = F(x) G(t)
	\\
	\\
	F(x) G''(t) = c^2 F''(x) G(t)
	\\
	\frac{F''(x)}{F(x)} =
	\frac{G''(t)}{c^2 G(t)} = k = -p^2
	\\
	F''(x) + p^2 F(x) = 0
	\qquad
	G''(t) + p^2 c^2 G(t) = 0
	\\
	\\
	F(x) = a \cos{p x} + b \sin{p x}
	\\
	F(0) = 0 = a \Rightarrow F(x) = \sin{p x}
	\\
	F'(x) = p \cos{p x}
	\\
	F'(L) = 0 = \cos{p x}
	\\
	p L = n \pi + \frac{\pi}{2},
	\qquad
	n \in \mathbb{N}
	\\
	p = \frac{(2 n + 1) \pi}{2 L}
	\\
	\\
	G(t) = A \cos{p c t} + B \sin{p c t}
	\\
	G_t(t) = -A p c \sin{p c t} + B p c \sin{p c t}
	\\
	G_t(0) = 0 = B p c \Rightarrow G(t) = A \cos{p c t}
	\\
	\\
	u_n(x, t) = A_n \sin{p_n x}\ \cos{p_n c t}
	\\
	u(x, t) = \sum_{n = 0}^\infty{A_n \sin{p_n x}\ \cos{p_n c t}}
	\\
	u(x, 0) = f(x) = \sum_{n = 0}^\infty{A_n \sin{p_n x}} \Rightarrow A_n = \frac{2}{L} \int_0^L{f(x) \sin{p_n x}\ dx}
\end{gather*}


\newpage


\section*{12.6}

\subsection*{21}


\begin{gather*}
	u_{xx} + u_{yy} = 0
	\\
	u(x, 24) = 25
	\qquad
	u(x, 0) = 0
	\qquad
	u(0, y) = 0
	\qquad
	u(24, y) = 0
	\\
	\\
	u_n = F(x) G(y)
	\qquad
	-\frac{F''(x)}{F(x)} = \frac{G''(y)}{G(y)} = k
	\\
	F''(x) + k F(x) = 0
	\qquad
	G''(y) - k G(y) = 0
	\qquad
	k = \left(\frac{n \pi}{24}\right)^2
	\\
	F(x) = \sin{\left(
		\frac{n \pi}{24} x
	\right)}
	\qquad
	G(y) = A_n \sinh{\left(
		\frac{n \pi}{24} y
	\right)}
	\\
	u(x, y) = \sum_{n = 1}^\infty{
		A_n \sinh{\left(
			\frac{n \pi}{24} y
		\right)}
		\sin{\left(
			\frac{n \pi}{24} x
		\right)}
	}
	\\
	u(x, 24) = 25 = \sum_{n = 1}^\infty{
		A_n \sinh{\left(
			n \pi
		\right)}
		\sin{\left(
			\frac{n \pi}{24} x
		\right)}
	}
	\\
	A_n \sinh{(n \pi)} = \frac{2}{24} \int_0^{24}{25 \sin{\left(
		\frac{n \pi}{24} x
	\right)}dx}
	\\
	A_n = \frac{25}{2 \sinh{(n \pi)}} \int_0^{24}{
		\sin{\left(\frac{n \pi}{24} x\right)} dx
	}
	=
	\frac{300 \left(1 - \cos{n \pi}\right)}{n \pi \sinh{n \pi}}
	\\
	\\
	u(x, y) = \sum_{n = 1}^\infty{
		\frac{300 \left(1 - \cos{n \pi}\right)}{n \pi \sinh{n \pi}}
		\sinh{\left(
			\frac{n \pi}{24} y
		\right)} \sin{\left(\frac{n \pi}{24} x\right)}
	}
\end{gather*}


\subsection*{23}


\begin{gather*}
	u_{xx} + u_{yy} = 0
	\\
	u(0, y) = 0
	\qquad
	u(24, y) = f(y)
	\qquad
	u_y(x, 0) = 0
	\qquad
	u_y(x, 24) = 0
	\\
	\\
	u_n = F(x) G(y)
	\qquad
	-\frac{F''(x)}{F(x)} = \frac{G''(y)}{G(y)} = k
	\\
	F''(x) + k F(x) = 0
	\qquad
	G''(y) - k G(y) = 0
	\qquad
	k = -\left(
		\frac{n \pi}{24}
	\right)^2
	\\
	F(x) = \sinh{\left(\frac{n \pi}{24} x\right)}
	\qquad
	G(y) = A \cos{\left(\frac{n \pi}{24} y\right)}
	\\
	u(x, y) = \sum_{n = 1}^\infty{
		A_n \sinh{\frac{n \pi}{24} x} \cos{\frac{n \pi}{24} y}
	}
	\\
	A_n = \frac{1}{12 \sinh{n \pi}} \int_0^{24}{f(y) \cos{\frac{n \pi}{24} y}\ dy}
\end{gather*}


\section*{12.7}

\subsection*{4}


\begin{gather*}
	u_t = c^2 u_{xx}
	\qquad
	u(x, 0) = f(x) = e^{-|x|}
	\\
	\\
	\fourier{u_t} = c^2 \fourier{u_{xx}}
	\\
	\hat u_t = -c^2 \omega^2 \hat u
	\\
	\hat u (\omega, t) = C(\omega) e^{-c^2 \omega^2 t}
	\\
	\hat u (\omega, 0) = \hat f(\omega) = C(\omega)
	\\
	\hat u (\omega, t) = \hat f(\omega) e^{-c^2 \omega^2 t}
	=
	\\
	\frac{\sqrt{2}}{\sqrt{\pi}} \frac{1}{1 + \omega} e^{-c^2 \omega^2 t}
	\\
	\\
	u(x, t) = \frac{1}{\sqrt{2 \pi}} \int_{-\infty}^\infty{
		\frac{\sqrt{2}}{\sqrt{\pi}} \frac{1}{1 + \omega} e^{-c^2 \omega^2 t} d\omega
	}
	=
	\\
	\\
	\frac{1}{\pi} \int_{-\infty}^\infty{
		\frac{1}{1 + \omega} e^{i x \omega - c^2 t \omega^2} d\omega
	}
\end{gather*}


\section*{13.1}

\subsection*{2}


\begin{gather*}
	z = x + i y = r e^{i \theta} = r \left(
		\cos{\theta} + i \sin{\theta}
	\right)
	\\
	i = 0 + i \cdot 1 = 1 \cdot e^{\frac{\pi}{2} i} =
	\cos{\frac{\pi}{2}} + i \sin{\frac{\pi}{2}}
	\\
	z \cdot i = r e^{i \theta} \cdot e^{\frac{\pi}{2} i} =
	r e^{\left(\theta + \frac{\pi}{2}\right) i}
\end{gather*}


\subsection*{5}


\begin{gather*}
	z = x + i y
	\\
	z\ \text{pure imaginary} \Leftrightarrow x = 0
	\\
	\bar z = -z \Leftrightarrow
	x - i y = -x - i y \Leftrightarrow
	\\
	x = -x \Leftrightarrow x = 0
\end{gather*}


\subsection*{6}


\begin{gather*}
	z_1 = r_1 e^{i \theta_1}, 
	\qquad
	z_2 = r_2 e^{i \theta_2}
	\\
	z_1 \cdot z_2 = r_1 \cdot r_2 e^{i \left(\theta_1 + \theta_2\right)} = 0 \Rightarrow
	\\
	|z_1 \cdot z_2| = r_1 \cdot r_2 = |0| = 0 \Rightarrow
	\\
	r_1 = 0 \vee r_2 = 0
\end{gather*}


\subsection*{9}


\begin{gather*}
	z_1 = -2 + 5 i
	\\
	z_1^2 = (-2 + 5 i)^2
	=
	2^2 - 2 \cdot 5 i + (5 i)^2
	=
	4 - 25 - 10 i = -21 - 10 i
	\\
	\text{Re} \left(z_1^2\right) = \text{Re} (-21 - 10 i) = -21
	\\
	\\
	(\text{Re } z_1)^2 = (-2)^2 = 4
\end{gather*}


\subsection*{14}


\begin{gather*}
	z_2 = 3 - i
	\\
	\frac{\bar z_1}{\bar z_2}
	=
	\frac{-2 - 5 i}{3 + i}
	=
	\frac{-2 - 5 i}{3 + i} \cdot \frac{3 - i}{3 - i}
	=
	\frac{-6 + 2 i - 15 i - 5}{9 + 1}
	=
	\frac{-11 - 13 i}{10} = -1.1 - 1.3 i
	\\
	\\
	\frac{z_1}{z_2}
	=
	\frac{-2 + 5 i}{3 - i} = -1.1 + 1.3 i
	\\
	\bar{\left(\frac{z_1}{z_2}\right)} = -1.1 - 1.3 i
\end{gather*}


\subsection*{16}


\begin{gather*}
	\frac{1}{z} = \frac{1}{x + i y}
	=
	\frac{1}{x + i y} \cdot \frac{x - i y}{x - i y}
	=
	\frac{x - i y}{x^2 + y^2}
	=
	\frac{x}{x^2 + y^2} - i \frac{y}{x^2 + y^2}
	\\
	\text{Im}\left(\frac{1}{z}\right) = \frac{y}{x^2 + y^2}
	\\
	\\
	\frac{1}{z^2} = \frac{1}{x^2 - y^2 + 2 i y}
	=
	\frac{1}{x^2 - y^2 + 2 i y} \cdot \frac{x^2 - y^2 - 2 i y}{x^2 - y^2 - 2 i y}
	=
	\\
	\frac{x^2 - y^2 - 2 i y}{\left(x^2 - y^2\right)^2 + 4 y^2}
	=
	\frac{x^2 - y^2 - 2 i y}{x^4 - 2 x^2 y^2 + y^4 + 4 y^2}
	\\
	\text{Im}\left(\frac{1}{z^2}\right) = \frac{2 y}{x^4 - 2 x^2 y^2 + y^4 + 4 y^2}
\end{gather*}

