\begin{center}
	\LARGE{\textbf{Ã˜ving 4}}
\end{center}


\section*{11.3}

\subsection*{14}


\begin{gather*}
	r(t) = \left\{
		\begin{matrix*}[l]
			-1	& -\pi < t < 0 \\ \\
			1	& 0 < t < \pi
		\end{matrix*}
	\right. \quad
	r(t + 2 \pi) = r(t)
	\\
	\\
	a_n = 0
	\quad
	b_n = \frac{2}{\pi} \int_0^\pi{\sin{n t}\ dt} =
	\\
	\frac{2}{\pi} \left[
		- \frac{1}{n} \cos{n t}
	\right]_0^\pi =
	\left\{
		\begin{matrix*}
			\frac{4}{\pi n}	& n\ \text{odd} \\
			0				& n\ \text{even}
		\end{matrix*}
	\right.
	\\
	\\
	r(t) = \sum_{n\ \text{odd}}^\infty{\frac{4}{\pi n} \sin{n t}}
	\\
	\\
	y = \sum_{n\ \text{odd}}^\infty{A_n \cos{n t} + B_n \sin{n t}}
	\\
	\\
	y'' + c y' + y = r(t)
	\\
	y_n = A_n \cos{n t} + B_n \sin{n t} \quad
	y_n' = -A_n n \sin{n t} + B_n n \cos{n t} \quad
	y_n'' = -A_n n^2 \cos{n t} - B_n n^2 \sin{n t}
	\\
	\\
	B_n - c A_n n - B_n n^2 = \frac{4}{\pi n} \quad
	A_n + c B_n n - A_n n^2 = 0
	\\
	A_n = \frac{4 c}{\pi \left(
		-n^4 + \left(
			c^2 + 2
		\right)
		n^2 - 1
	\right)} \quad
	B_n = \frac{4 n^2 - 4}{\pi \left(
		-n^5 + \left(
			c^2 + 2
		\right)
		n^3 - n
	\right)}
	\\
	\\
	\plot{Figurer/f0.tikz}{8}{6}
\end{gather*}


\newpage


\subsection*{16}


\begin{gather*}
	r(t) = \left\{
		\begin{matrix*}
			t		& -\frac{\pi}{2} < t < \frac{\pi}{2} \\ \\
			\pi - t	& \frac{\pi}{2} < t < \frac{3 \pi}{2}
		\end{matrix*}
	\right.
	\\
	\\
	r(t) \quad \text{odd} \Rightarrow a_n = 0
	\\
	b_n = \int_{-\frac{\pi}{2}}^{\frac{\pi}{2}}{t \sin{n t}\ dt} +
	\int_{\frac{\pi}{2}}^{\frac{3 \pi}{2}}{(\pi - t) \sin{n t}\ dt} =
	\\
	\frac{4}{n^2} (-1)^\frac{n - 1}{2} \quad \forall\ n\ \text{odd}
	\\
	\\
	y = \sum_{n\ \text{odd}}^\infty{A_n \cos{n t} + B_n \sin{n t}}
	\\
	\\
	y'' + c y' + y = r(t)
	\\
	y_n = A_n \cos{n t} + B_n \sin{n t} \quad
	y_n' = -A_n n \sin{n t} + B_n n \cos{n t} \quad
	y_n'' = -A_n n^2 \cos{n t} - B_n n^2 \sin{n t}
	\\
	\\
	B_n - c A_n n - B_n n^2 = \frac{4}{n^2} (-1)^\frac{n - 1}{2} \quad
	A_n + c B_n n - A_n n^2 = 0
	\\
	\\
	A_n = \frac{4 c}{n^5 + \left(
		c^2 - 2
	\right) n^3 + n} \quad
	B_n = \frac{4 \left(
		n^2 - 1
	\right)}{n^6 + \left(
		c^2 - 2
	\right) n^4 + n^2}
	\\
	\\
	\plot{Figurer/f1.tikz}{8}{6}
\end{gather*}


\newpage


\section*{11.4}

\subsection*{3}


\begin{gather*}
	f(x) = \left|
		x
	\right|
	\quad
	-\pi < x < \pi
	\quad
	f(x + 2 \pi) = f(x)
	\\
	\\
	b_n = 0
	\quad
	a_0 = \frac{1}{\pi} \int_0^\pi{x dx} = \frac{\pi}{2}
	\\
	a_n = \frac{2}{\pi} \int_0^\pi{x \cos{n x}\ dx} =
	\frac{2}{n} \cancel{\sin{n \pi}} + \frac{2}{\pi n^2} \left(
		\cos{n \pi} - 1
	\right) =
	-\frac{4}{\pi n^2} \quad n\ \text{odd}
	\\
	\\
	F(x) = \frac{\pi}{2} - \frac{4}{\pi} \sum_{n\ \text{odd}}^N{\frac{1}{n^2} \cos{n x}} =
	\frac{\pi}{2} - \frac{4}{\pi} \cos{x} - \frac{4}{9 \pi} \cos{3 x} - \frac{4}{25 \pi} \cos{5 x} - ...
	\\
	\\
	E^* = \int_{\pi}^\pi{x^2 dx} - \pi \left[
		2 \left(
			\frac{\pi}{2}
		\right)^2
		+ \sum_{n\ \text{odd}}^N{\left(
			\frac{-4}{\pi n^2}
		\right)^2}
	\right] =
	\\
	\frac{1}{6}\pi^3 - \frac{16}{\pi} \sum_{n\ \text{odd}}^N{\frac{1}{n^4}} =
	\frac{1}{6}\pi^3 - \frac{16}{\pi} \left(
		\frac{1}{1} + \frac{1}{81} + \frac{1}{625} + ...
	\right)
	\\
	\\
	E_{1-5}^* = 0.0748, 0.0119, 0.00373
\end{gather*}


\subsection*{5}


\begin{gather*}
	f(x) = \left\{
		\begin{matrix*}[l]
			-1	& -\pi < x < 0 \\ \\
			1	& 0 < x < \pi
		\end{matrix*}
	\right. \quad
	f(x + 2 \pi) = f(x)
	\\
	\\
	a_n = 0
	\quad
	b_n = \frac{2}{\pi} \int_0^\pi{\sin{n x}\ dx} = \left\{
		\begin{matrix*}[l]
			\frac{4}{\pi n}	& n\ \text{odd} \\
			0				& n\ \text{even}
		\end{matrix*}
	\right.
	\\
	\\
	F(x) = \frac{4}{\pi} \sum_{n\ \text{odd}}^N{\frac{1}{n} \sin{n x}} =
	\frac{4}{\pi} \left(
		\sin{x} + \frac{1}{3} \sin{3 x} + \frac{1}{5} \sin{5 x} + ...
	\right)
	\\
	\\
	E^* = 2 \int_0^\pi{dx} - \pi \sum_{n\ \text{odd}}^N{\left(
		\frac{4}{\pi n}
	\right)^2} = 
	2 \pi - \frac{16}{\pi} \sum_{n\ \text{odd}}^N{\frac{1}{n^2}}
	\\
	\\
	E_{1-5}^* = 1.19, 0.624, 0.421
\end{gather*}


\subsection*{6}


Square errors for discontious functons are larger than for continous functions.


\subsection*{11}


\begin{gather*}
	\text{From 11.4.5 we have} 
	\\
	E^* = 2 \pi - \frac{16}{\pi} \sum_{n\ \text{odd}}^N{\frac{1}{n^2}}
	\\
	\lim_{N \rightarrow \infty}{E^*} = 0
	\\
	2 \pi - \frac{16}{\pi} \sum_{n\ \text{odd}}^\infty{\frac{1}{n^2}} = 0
	\\
	\sum_{n\ \text{odd}}^\infty{\frac{1}{n^2}} = 2 \pi \cdot \frac{\pi}{16} = \frac{\pi^2}{8}
	\\
	\text{First few partial sums: }
	\\
	1, 1.1111, 1.1511, 1.1715, 1.1839
\end{gather*}


\section*{Denne}


\begin{gather*}
	\sum_{\underset{n\neq 0}{n = \infty}}^\infty{\frac{e^{i n x}}{2 n^2}} =
	\sum_{n = 1}^\infty{\frac{1}{2 n^2} \left(
		e^{i n x} + e^{- i n x}
	\right)} =
	\\
	\sum_{n = 1}^\infty{\frac{1}{2 n^2} \left(
		\cos{n x} + i \sin{n x} + \cos{n x} - i \sin{n x}
	\right)} =
	\\
	\sum_{n = 1}^\infty{\frac{1}{n^2} \cos{n x}} \quad \Rightarrow \quad
	a_0 = 0, \quad a_n = \frac{1}{n^2}, \quad b_n = 0
\end{gather*}
